\section{Exercise 1}
\paragraph{a)}\label{par:a}
\begin{align}
u_t + 7u_x=0,&\label{eq:1a}\\
u \rightarrow u(x,t),&\\
u_0 \rightarrow u(0,t).&
\end{align}
Introduce curve in space time with parametrisation $u(x(s),t(s))$. Using the chain rule we can calculate the total derivative of $u$  by the parameter $s$
\begin{align}
\der{}{s}u(x(s),t(s)) = \der{x}{s}\pder{u}{x} + \der{t}{s}\pder{u}{t}
\end{align}
When choosing parametrisation that fulfil $\der{t}{s} = 1$ and $\der{x}{s}=7$ we see, that the left hand side  of  \cref{eq:1a} can be written as $\der{}{s}u(x(s),t(s))=0$.
So along the characteristics we can reduce the  PDE to three ODE's 
\begin{align}
\der{t}{s} &= 1,\\
\der{x}{s}&=7,\\
\der{}{s}u&=0.
\end{align}
We can easily solve them
\begin{align}
t=s +t_0,\\
x = 7s + x_0,\label{eq:1a_xs}\\
u(x,t) = u(x_0, 0) =u_0(x_0)\label{eq:1a_u_u0} .
\end{align}
If we set $t_0=0$ we get $t=s$. Plugging this into \cref{eq:1a_xs} we arrive at an equation for the charachteristics 
\begin{align}
x(t) = 7t + x_0.\label{eq:1a_charch_curve}
\end{align}
A plot can be seen in \cref{fig:1aplot}.
Solving this for $x_0$ and plugging into \cref{eq:1a_u_u0} gives us the general solution
\begin{align}
u(x,t)=u_0(x_0)=u_0(x-7t).
\end{align}

\paragraph{b)}
\begin{align}
u_t - 2u_x +3u=0,&\label{eq:1a}\\
u \rightarrow u(x,t),&\\
u_0 \rightarrow u(0,t).&
\end{align}
We use the same reasoning as in \cref{par:a} to arrive at the equations
\begin{align}
\der{t}{s} &= 1,\\
\der{x}{s}&=-2,\\
\der{}{s}u&+3u=0.\label{eq:1b_difu}
\end{align}

The first two equations can again be solved by simple integration. For the last we use the exponential ansatz $u(x(s),t(s)) = u_0(x_0)\cdot e^{a\cdot s}$. Plugging this into \cref{eq:1b_difu} results in the equation
\begin{align}
 u_0(x_0)\cdot e^{a\cdot s}\cdot(a+3) = 0.
\end{align}
For non trivial initial conditions we thus find $a=-3$. The solutions to the three equations are given by 
\begin{align}
t(s)&=s+t_0,\\
x(s)&=-2s+x_0,\\
u(x(s),t(s))&=u_0(x_0)\cdot e^{-3s}
\end{align}
If we set $t_0=0$ we get $t=s$, the charachteristic curves then become
\begin{align}
x(t)=-2t+x_0.\label{eq:1b_charch_curve}
\end{align}
A plot can be found in \cref{fig:1bplot}.
The full solution is then together with $x_0=x+2t$
\begin{align}
u(x(t),t)=u_0(x+2t)\cdot e^{-3t}.
\end{align}
\begin{figure}
\subfloat[Charachteristic curves given by \cref{eq:1a_charch_curve} with different starting conditions $x_0$.\label{fig:1aplot}]{\includegraphics[width=0.49\textwidth]{CharachteristicCurve_1a.pdf}}
\hfill
\subfloat[Charachteristic curves given by \cref{eq:1b_charch_curve} with different starting conditions $x_0$.\label{fig:1bplot}]{\includegraphics[width=0.49\textwidth]{CharachteristicCurve_1b.pdf}}
\end{figure}